
\documentclass[12pt]{article}
\usepackage[margin=1in]{geometry}

\input{../../variables.tex}

\title{%
    \Huge Miscellaneous \\
}
\date{2024-01-5}
\author{Michael Saba}

\begin{document}
    \pagenumbering{gobble}
    \maketitle
    \newpage
    \pagenumbering{arabic}

    \section*{I. Square Root of Tangent Integral}
    \[
        F(x) = \int \sqrt{\tan{(x)}} \, dx 
    \]
    \[
        = \begin{bmatrix}
            u = \sqrt{\tan{(x)}} \\
            du = \frac{\sec^2{(x)}}{2\sqrt{\tan{(x)}}} \\
            \frac{2u}{u^4 + 1}du = dx
        \end{bmatrix} = \int \frac{2u^2}{u^4 + 1} \, du 
    \]
    \[
        = \int \frac{u^2 + u^2 + 1 - 1}{u^4 + 1} \, du 
    \]
    \[
        = \int \frac{u^2 + 1}{u^4 + 1} \, du 
        + \int \frac{u^2 - 1}{u^4 + 1} \, du 
    \]
    \[
        = \int \left(\frac{1 + \frac{1}{u^2}}{u^2 
        + \frac{1}{u^2}} + \frac{1 - \frac{1}{u^2}}{u^2 
        + \frac{1}{u^2}}\right) \, du 
    \]
    \[
        = \int \left(\frac{1 + \frac{1}{u^2}}{u^2 
        + \frac{1}{u^2} + 2 - 2} + \frac{1 - \frac{1}{u^2}}
        {u^2 + \frac{1}{u^2} + 2 - 2}\right) \, du 
    \]
    \[
        = \int \left(\frac{1 + \frac{1}{u^2}}
        {(u - \frac{1}{u})^2 + 2} + \frac{1 - \frac{1}{u^2}}
        {(u + \frac{1}{u})^2 - 2}\right) \, du 
    \]
    \[
        = \begin{bmatrix}
            v = u - \frac{1}{u} \\
            w = u + \frac{1}{u} \\
            dv = (1 + \frac{1}{u^2}) \, du \\
            dw = (1 - \frac{1}{u^2}) \, du
        \end{bmatrix}
        = \int \frac{dv}{v^2 + 2} + \int \frac{dw}{w^2 - 2} 
    \]
    \[
        = \frac{1}{2}\int \frac{dv}{\left(\frac{v}{\sqrt{2}}\right)^2 + 1} 
        + \frac{1}{2}\int \frac{dw}{\left(\frac{w}{\sqrt{2}}\right)^2 - 1} 
    \]
    \[
        = \frac{\sqrt{2}}{2}\arctan{\left(\frac{v}{\sqrt{2}}\right)} 
        + \frac{1}{2}\int \frac{dw}{\left(\frac{w}{\sqrt{2}} - 1\right)
        \left(\frac{w}{\sqrt{2}} + 1\right)} 
    \]
    \[
        = \frac{\sqrt{2}}{2}\arctan{\left(\frac{v}{\sqrt{2}}\right)} 
        + \frac{1}{2}\int \left(\frac{A}{\frac{w}{\sqrt{2}} - 1} + \frac{B}
        {\frac{w}{\sqrt{2}} + 1}\right) \, dw 
    \]
    \[
        \begin{cases}
            \sfrac{A}{\sqrt{2}} +  \sfrac{B}{\sqrt{2}} = 0 
            \implies A = -B \\
            A - B = 1 \implies A = 1 + B  \\
        \end{cases}
    \]
    \[
        \text{So } -B = 1 + B
        \text{, which means that } B = -\dfrac{1}{2}
        \text{ and } A = \dfrac{1}{2}
    \]
    \[
        = \frac{\sqrt{2}}{2}\arctan{\left(\frac{v}{\sqrt{2}}\right)} 
        + \frac{1}{4}\int \left(\frac{1}{\frac{w}{\sqrt{2}} - 1} - \frac{1}
        {\frac{w}{\sqrt{2}} + 1}\right) \, dw 
    \]
    \[
        = \frac{\sqrt{2}}{2}\arctan{\left(\frac{v}{\sqrt{2}}\right)} 
        + \frac{\sqrt{2}}{4} \left(\ln{\left|\frac{w}{\sqrt{2}} - 1\right|} 
        - \ln{\left|\frac{w}{\sqrt{2}} + 1\right|}\right) 
    \]
    \[
        = \frac{\sqrt{2}}{2}\arctan{\left(\frac{u + \frac{1}{u}}{\sqrt{2}}
        \right)} + \frac{\sqrt{2}}{4} \left(\ln{\left|\frac{u + \frac{1}{u} 
        - \sqrt{2}}{\sqrt{2}}\right|} - \ln{\left|\frac{u + \frac{1}{u} 
        + \sqrt{2}}{\sqrt{2}}\right|}\right) 
    \]
    \[
        = \dfrac{\sqrt{2}}{2}\arctan{ 
            \left(
                \dfrac{ \sqrt{\tan{(x)}} 
                - \sfrac{1}{ \sqrt{\tan{(x)}}}}{\sqrt{2}} 
            \right)
        }
        + \dfrac{\sqrt{2}}{4} 
        \ln{\left| 
            \dfrac{\sqrt{\tan{(x)}} + \sfrac{1}{ \sqrt{\tan{(x)}}} - \sqrt{2}}
            {\sqrt{\tan{(x)}} + \sfrac{1}{ \sqrt{\tan{(x)}}} + \sqrt{2}}
        \right|}
    \]

    \newpage

    \subsection*{II. Differential Equation using Laplace Transform}
    \[
        y'' - y' - 2y  = 2t + 1 \qquad y(0) = 1, \, y'(1) = 2
    \]
    \[
        \laplace{y'' - y' - 2y} = \laplace{2t+1}
    \]
    \[
        \laplace{y''} - \laplace{y'} - \laplace{2y} 
        = 2\laplace{t} + \laplace{1}
    \]
    \[
        \text{Taking } Y(s)
        \text{ to be the laplace transform } \laplace{y(t)}
    \]
    \[
        (s^2Y(s) - sy(0) - y'(0))
        - (sY(s) - y(0)) - 2Y(s)
        = \sfrac{2}{s^2} - \sfrac{1}{s}
    \]
    \[
        (s^2-s-2)Y(s) - s - 2 - 1 = \dfrac{2}{s^2} - \dfrac{1}{s}
    \]
    \[
        (s^2-s-2)Y(s) = \dfrac{2}{s^2} - \dfrac{1}{s} + s + 1
    \]
    \[
        (s^2-s-2)Y(s) = \dfrac{s^3 + s^2 + s + 2}{s^2}
    \]
    \[
        Y(s) = \dfrac{s^3 + s^2 + s + 2}{s^2(s^2-s-2)}
    \]
    \[
        Y(s) = \dfrac{s^3 + s^2 + s + 2}{s^2(s-2)(s+1)}
        = \dfrac{A}{s^2} + \dfrac{B}{s} + \dfrac{C}{s-2} + \dfrac{D}{s+1}
    \]
    \[
        \begin{cases}
            -2A = 2 \implies A = -1 \\
            -A - 2B = 1 \implies -2B = (1-1) \implies B = 0 \\
            A - B + C -2D = 1 \implies C - 2D = 2 \\
            B + C + D = 1 \implies C + D = 1 \\
        \end{cases}
    \]
    \[ \text{Subtracting the fourth line from the third, we get } \]
    \[
        -3D = 1 \implies D = -\dfrac{1}{3}
        \implies C - \dfrac{1}{3} = 1 \implies C = \dfrac{4}{3}
    \]
    \[
        Y(s) = -\dfrac{1}{s^2} + \dfrac{\sfrac{4}{3}}{s-2}
        - \dfrac{\sfrac{1}{3}}{s+1}
    \]
    \[
        \invlaplace{Y(s)} = -\invlaplace{\dfrac{1}{s^2}} 
        + \dfrac{4}{3}\invlaplace{\dfrac{1}{s-2}}
        - \dfrac{1}{3}\invlaplace{\dfrac{1}{s+1}}
    \]
    \[
        y(t) = -t + \dfrac{4e^{2t}}{3} - \dfrac{e^{-t}}{3}
    \]

    

\end{document}
