
\documentclass[12pt]{article}
\usepackage[margin=1in]{geometry}

\input{../../../../variables.tex}

\title{%
    \Huge Book of Proof \\
    \large by \\
    \Large Richard Hammack \\~\\
    \huge Part 2: How to Prove a Conditional Statement \\
    \LARGE Chapter 4: Direct Proof
}
\date{2024-03-17}
\author{Michael Saba}

\begin{document}
    \pagenumbering{gobble}
    \maketitle
    \newpage
    \setlength{\parindent}{0pt}
    \pagenumbering{arabic}

    For questions 1 - 28, we have to use a direct proof. \\

    \section*{Exercise 1}
    Proof that if $x$ is even,
    then $x^2$ is even: \\
    Suppose that $x$ is an even integer.
    Then $x = 2n$ for some $n \in \zbb$.
    So $x^2 = (2n)^2 = (2n)^2 = 4n^2 = 2(2n^2)$
    where $2n^2$ is an integer.
    So $x^2$ is even.

    \section*{Exercise 2}
    Proof that if $x$ is odd,
    then $x^3$ is odd: \\
    Suppose that $x$ is an odd integer.
    Then $x = 2n+1$ for some $n \in \zbb$.
    So
    \[ x^3 = (2n+1)^3 = 8n^3 + 4n^2 + 2n + 1 = 2(4n^3 + 2n^2 + n) + 1 \]
    where $4n^3 + 2n^2 + n$ is an integer.
    So $x^3$ is odd. \\

    \section*{Exercise 3}
    Proof that if $a$ is odd,
    then $a^3 + 3a + 5$ is odd: \\
    Suppose that $a$ is an odd integer.
    Then $a = 2n+1$ for some $n \in \zbb$.
    So 
    \[ a^3 + 3a + 5 = (2n+1)^3 + 3(2n+1) + 5 \]
    \[ = 8n^3 + 4n^2 + 8n + 9 = 2(4n^3 + 2n^2 + 4n + 4) + 1 \]
    where $4n^3 + 2n^2 + 4n + 4$ is an integer.
    So $a^3 + 3a + 5$ is odd. \\

    \section*{Exercise 4}
    Proof that for $x, y \in \zbb$,
    $xy$ is odd if $x$ and $y$ are odd: \\
    Suppose that $x$ and $y$ are odd integers.
    Then $x = 2n+1$ and $y = 2m+1$ for some $n, m \in \zbb$.
    So 
    \[ xy = (2n+1)(2m+1) = 4nm + 2n + 2m + 1 = 2(2nm + n + m) + 1\]
    where $2nm + n + m$ is an integer.
    So $xy$ is odd. \\

    \section*{Exercise 5}
    Proof that for $x, y \in \zbb$,
    $xy$ is even if $x$ is even: \\
    Suppose that $x$ and $y$ are integers
    such that $x$ is even. 
    Then $x = 2n$ and $y = 2m+1$ for some $n, m \in \zbb$.
    So 
    \[ xy = (2n)(2m+1) = 4nm + 2n = 2(2nm + n)\]
    where $2nm + n$ is an integer.
    So $xy$ is even. \\

    \section*{Exercise 6}
    Proof that for $a, b, c \in \zbb$,
    if $a \mid b$ and $a \mid c$,
    then $a \mid (b+c)$: \\
    Suppose that $a, b, c$ are integers
    such that $a \mid b$ and $a \mid c$.
    Then $b = an$ and $c = am$ for some $n, m \in \zbb$.
    So $b+c = an + am = a(n + m)$,
    which means that $a \mid (b+c)$. \\

    \section*{Exercise 7}
    Proof that for $a, b \in \zbb$,
    if $a \mid b$,
    then $a^2 \mid b^2$: \\
    Suppose that $a, b$ are integers
    such that $a \mid b$.
    Then $b = an$ for some $n \in \zbb$.
    So $b^2 = (an)^2 = a^2n^2$,
    which means that $a^2 \mid b^2$. \\

    \section*{Exercise 8}
    Proof that for $a \in \zbb$,
    if $5 \mid 2a$,
    then $5 \mid a$: \\
    Suppose that $a \in \zbb$
    such that $5 \mid 2a$.
    Then $2a = 5n$ for some $n \in \zbb$.
    So $5n$ must be even,
    which means that it contains a factor of $2$.
    But $5$ is prime and can't be factored further,
    so $2$ must be a factor of $n$, making it even,
    such that $n = 2m$ for some $m \in \zbb$.
    So $2a = 5 \cdot 2m$,
    which means that $a = 5m$.
    So $5 \mid a$. \\

    \section*{Exercise 9}
    Proof that for $a \in \zbb$,
    if $7 \mid 4a$,
    then $7 \mid a$: \\
    Suppose that $a \in \zbb$
    such that $7 \mid 4a$.
    Then $4a = 7n$ for some $n \in \zbb$.
    So $7n$ must have a factor of $4$.
    But $7$ is prime and can't be factored further,
    so $4$ must be a factor of $n$,
    such that $n = 4m$ for some $m \in \zbb$.
    So $4a = 7 \cdot 4m$,
    which means that $a = 7m$.
    So $7 \mid a$. \\

    \section*{Exercise 10}
    Proof that for $a, b \in \zbb$,
    if $a \mid b$,
    then $a \mid (3b^3 - b^2 + 5b)$: \\
    Suppose that $a \in \zbb$
    such that $a \mid b$.
    Then $b = an$ for some $n \in \zbb$.
    So 
    \[ 3b^3 - b^2 + 5b = 3(an)^3 - (an)^2 + 5(an)
    = 3a^3n^3 - a^2n^2 + 5an = a(3a^2n^3 - an^2 + 5n) \]
    where $3a^2n^3 - an^2 + 5n$,
    which means that $a \mid (3b^3 - b^2 + 5b)$. \\

    \section*{Exercise 11}
    Proof that for $a, b, c, d \in \zbb$,
    if $a \mid b$ and $c \mid d$,
    then $ac \mid bd$: \\
    Suppose that $a, b, c, d \in \zbb$
    such that $a \mid b$ and $c \mid d$.
    Then $b = an$ and $d = cm$ for some $a, c \in \zbb$.
    So $bd = ancm = ac(nm)$,
    which means that $ac \mid bd$. \\

    \section*{Exercise 12}
    Proof that for $x \in \rbb$,
    if $0 < x < 4$,
    then $\dfrac{4}{x(4-x)} \geqslant 1$: \\
    Suppose that $x \in \rbb$
    such that $0 < x < 4$.
    We know that $(x-2)^2 \geqslant 0$ since all squares are positive.
    We can then develop the term and get
    that $x^2 - 4x + 4 \geqslant 0$,
    which means that $4 \geqslant 4x - x^2$,
    which in turn means that $4 \geqslant x(4 - x)$.
    We can thus conclude that $\dfrac{4}{x(4-x)} \geqslant 1$
    as the numertaor is larger than the denominator.
    (Note that this ended up being the case
    regardless of the fact that $0 < x < 4$). \\

    \section*{Exercise 13}
    Proof that for $x, y \in \rbb$,
    if $x^2+5y = y^2+5x$,
    then $x = y$ or $x+y = 5$: \\
    Suppose that $x, y \in \rbb$
    such that $x^2+5y = y^2+5x$.
    Then $x^2 - y^2 = 5x - 5y$,
    which we can restructure to get $(x+y)(x-y) = 5(x - y)$.
    If $x-y$ is $0$,
    then both sides of the equations are $0$,
    and it implies that $x = y$.
    On the other hand, if $x-y \neq 0$,
    then we can simplify by $x-y$,
    and get that $x+y = 5$. \\
    So either $x = y$ or $x+y = 5$. \\

    \section*{Exercise 14}
    Proof that if $n \in \zbb$,
    then $5n^2 + 3n + 7$ is odd: \\
    Suppose that $n \in \zbb$.
    We know that $n$ is awlays either even or odd,
    so if we can prove the statement for both cases,
    we've then covered all of our bases. \\
    If $n$ is even,
    then $n = 2m$ for some $m \in \zbb$.
    This means that 
    \[ 5n^2 + 3n + 7 = 5(2m)^2 + 3(2m) + 7 = 20m^2 + 6m + 7
    = 2(10m^2 + 3m + 3) + 1 \]
    where $10m^2 + 3m + 3$ is an integer,
    which means that $5n^2 + 3n + 7$ is odd. \\
    On the other hand, if $n$ is odd,
    then $n = 2p + 1$ for some $p \in \zbb$.
    This means that 
    \[ 5n^2 + 3n + 7 = 5(2p+1)^2 + 3(2p+1) + 7
    = 20(4p^2 + 4p + 1) + 6(2p+1) + 7 \]
    \[ = 80p^2 + 92p + 33
    = 2(40p^2 + 46p + 16) + 1 \]
    where $40p^2 + 46p + 16$ is an integer,
    which means that $5n^2 + 3n + 7$ is odd. \\

    \section*{Exercise 15}
    Proof that if $n \in \zbb$,
    then $n^2 + 3n + 4$ is even: \\
    Suppose that $n \in \zbb$.
    We know that $n$ is awlays either even or odd,
    so if we can prove the statement for both cases,
    we've then covered all of our bases. \\
    If $n$ is even,
    then $n = 2m$ for some $m \in \zbb$.
    This means that 
    \[ n^2 + 3n + 4 = (2m)^2 + 3(2m) + 4 = 4m^2 + 6m + 4
    = 1(2m^2 + 3m + 2) \]
    where $2m^2 + 3m + 2$ is an integer,
    which means that $n^2 + 3n + 4$ is even. \\
    On the other hand, if $n$ is odd,
    then $n = 2p + 1$ for some $p \in \zbb$.
    This means that 
    \[ n^2 + 3n + 4 = (2p+1)^2 + 3(2p+1) + 4 = 4m^2 + 10m + 8
    = 2(2m^2 + 5m + 4) \]
    where $2m^2 + 5m + 4$ is an integer,
    which means that $n^2 + 3n + 4$ is even. \\

    \section*{Exercise 16}
    Proof that for $x, y \in \zbb$,
    if $x$ and $y$ have the same parity,
    then $x+y$ is even: \\
    Suppose that $x, y \in \zbb$. \\
    If $x$ and $y$ are both even,
    then $x = 2n$ and $y=2m$ for some $n, m \in \zbb$.
    So $x+y = 2n + 2m = 2(n+m)$
    where $n+m$ is an integer,
    so $x+y$ is even. \\
    On the other hand, 
    if $x$ and $y$ are both odd,
    then $x = 2p+1$ and $y=2q+1$ for some $p, q \in \zbb$.
    So $x+y = 2p+1 + 2q+1 = 2(p+q+1)$
    where $p+q+1$ is an integer,
    so $x+y$ is even. \\

    \section*{Exercise 17}
    Proof that for $x, y \in \zbb$,
    if $x$ and $y$ have opposite parity,
    then $xy$ is even: \\
    Suppose that $x, y \in \zbb$
    such that they have opposite parity.
    We can assume, without loss of generality,
    that $x$ is even and $y$ is odd
    (the prove would be the same otherwise). 
    Then $x = 2n$ and $y=2m+1$ for some $n, m \in \zbb$.
    So $xy = 2n(2m+1) = 4nm + 2n = 2(2nm + n)$
    where $2nm + n$ is an integer,
    so $xy$ is even. \\

    \section*{Exercise 18}
    Proof that for $x, y \in \rbb$ where $x, y > 0$,
    if $x > y$,
    then $x^2 < y^2$: \\
    Suppose that $x, y \in \rbb$
    such that $x, y > 0$ and $x > y$.
    Since $x > 0$,
    we can multiply both sides of the equation by $x$
    without changing the direction of the operator,
    arriving at $x^2 > xy$.
    Likewise, since $y > 0$,
    we can multiply both sides of the equation by $y$
    without changing the direction of the operator,
    arriving at $xy > y^2$.
    So since $x^2 > xy > y^2$,
    it follows that $x^2 > y^2$. \\
   
    \section*{Exercise 19}
    Proof that for $a, b, c \in \zbb$,
    if $a^2 \mid b$ and $b^3 \mid c$,
    then $a^6 \mid c$: \\
    Suppose that $a, b, c \in \zbb$
    such that $a^2 \mid b$ and $b^3 \mid c$.
    Then $b = a^2n$ and $c = b^3m$ for some $n, m \in \zbb$.
    So $c = (a^2n)^3m = a^6n^3m$
    where $n^3m$ is an integer.
    This means that $a^6 \mid c$. \\

    \section*{Exercise 20}
    Proof that for $a \in \zbb$,
    if $a^2 \mid a$, 
    then $a \in \{-1, 0, 1\}$: \\
    Suppose that $a \in \zbb$
    such that $a^2 \mid a$.
    Then $a = a^2n$ for some $n \in \zbb$. \\
    If $a = 0$, the the equation holds. \\
    But if $a \neq 0$,
    then we could simplifty by $a$,
    and get that $1 = an$,
    which means that $n = \sfrac{1}{a}$,
    (where $a$ can be the denominator since we assumed $a \neq 0$).
    Since $n$ is an integer,
    it must be that $a = \pm 1$. \\
    So $a = 0$ or $a = 1$ or $1 = -1$,
    which means that $a \in \{-1, 0, 1\}$. \\

    \section*{Exercise 21 $***$}
    Proof that if $p$ is prime and $k \in \zbb$
    such that $0 < k < p$,
    then $p \mid \comb{p}{k}$: \\
    Suppose that $p$ is prime and $k \in \zbb$
    such that $0 < k < p$.
    Then 
    \[ \comb{p}{k} = \dfrac{p!}{k!(p-k)!} \]
    Since $p > k$ and $p > p - k$,
    and since $p$ is prime
    (meaning it is not the combination of several smaller factors),
    we conclude that the factor $p$ does not appear in $k!$ or $p-k!$.
    We know that $\dfrac{p!}{k!(p-k)!}$ is an integer,
    which means that $k!(p-k)!$ appear as factors in $p!$.
    But since $p$ as a factor does not appear in $k!$ or $(p-k)!$,
    we assert that $p$ and $k!(p-k)!$ have no factors in common.
    We know that $p! = p(p-1)!$,
    so since $k!(p-k)! \mid p!$
    and $p$ and $k!(p-k)!$ have no factors in common,
    it must be that $k!(p-k)!$ is a factor in $(p-1)!$,
    which means that $k!(p-k)! \mid (p-1)!$. \\
    So 
    \[ \comb{p}{k} = p\dfrac{(p-1)!}{k!(p-k)!} \]
    where
    \[ \dfrac{(p-1)!}{k!(p-k)!} \]
    is an integer.
    This means that $p \mid \comb{p}{k}$. \\

    \section*{Exercise 22}
    Proof that if $n \in \nbb$,
    then $n^2 = 2(\comb{n}{2}) + \comb{n}{1}$: \\
    Suppose that $n \in \nbb$ (a positive integer). \\
    We will consider first the case where $n = 1$,
    where $\comb{n}{1} = \comb{1}{1} = 1$
    and $\comb{n}{2} = \comb{1}{2} = 0$
    (there is no way to choose $2$ out of $1$).
    So $n^2 = 1^2 = 1$,
    and $2(\comb{n}{2}) + \comb{n}{1} = 0 + 1 = 1$,
    which means that $n^2 = 2(\comb{n}{2}) + \comb{n}{1}$. \\
    On the other hand,
    if $n \geqslant 2$,
    then 
    \[ \comb{n}{1} = \comb{n}{1} = n \]
    (there are exactly $n$ ways to choose a single element from $n$).
    and
    \[ \comb{n}{2} = \dfrac{n!}{2!(n-2)!}
    = \dfrac{n(n-1)}{2} \].
    So we have
    \[ 2(\comb{n}{2}) + \comb{n}{1} = n(n-1) + n = n^2 + n - n = n^2 \]
    which completes the proof. \\

    \section*{Exercise 23 $***$}
    Proof that if $n \in \nbb$,
    then $\comb{2n}{n}$ is even: \\
    Suppose that $n \in \nbb$.
    Thwn $\comb{2n}{n}$ is the number of ways we can choose $n$
    numbers out of $2n$.
    Everytime we choose $n$ numbers,
    we effectively build a set $X_i$ containing these numbers.
    Then all the numbers we did not pick will be in a set $\olsi{X_i}$.
    As such, we could pair each set $X_i$,
    with its compelement $\olsi{X_i}$,
    where $\olsi{X_i}$ has a length of $n$ as well.
    Since $\olsi{X_i}$ is itself
    a way to choose $n$ numbers from $2n$,
    it will contribute a combination in $\comb{2n}{n}$.
    Since each combination $X_i$ in $\comb{2n}{n}$ can be paired
    with another combination in $\comb{2n}{n}$,
    we conclude that $\comb{2n}{n}$ must be even. \\

    \section*{Exercise 24}
    Proof that for $n \in \zbb$,
    if $n \geqslant 2$,
    then $n! + 2, n! + 3 \dots n! + n$ are all compositie: \\
    Suppose that $n \in \zbb$
    such that $n \geqslant 2$,
    Then for $m \in \zbb$ 
    such that $2 \leqslant m \leqslant n$,
    we will have
    \[ n! = 2 \cdot 3 \dots m  \dots (n-1) \cdot n \]
    Then
    \[ n! + m = 2 \cdot 3 \dots m  \dots (n-1) \cdot n + m
    =  m (2 \cdot 3 \dots m - 1 \cdot m + 1  \dots (n-1) \cdot n) \]
    Since both $m$
    and $(2 \cdot 3 \dots m - 1 \cdot m + 1  \dots (n-1) \cdot n)$
    are integers larger than $1$,
    this shows that $n! + m$ is composite. \\

    \section*{Exercise 25}
    Proof that for $a, b, c \in \zbb$,
    if $c \leqslant b \leqslant a$,
    then $\comb{a}{b} \times \comb{b}{c}
    = \comb{a}{b-c} \times \comb{a-b+c}{b}$: \\
    Suppose that $a, b, c \in \zbb$
    such that $c \leqslant b \leqslant a$.
    Then
    \[ \comb{a}{b} \times \comb{b}{c} \]
    \[ = \dfrac{a!}{b!(a-b)!}\dfrac{b!}{c!(b-c)!} \]
    \[ = \dfrac{a!}{(a-b)!(b-c)!c!} \]
    Which means that
    \[ \comb{a}{b-c} \times \comb{a-b+c}{c} \]
    \[ = \dfrac{a!}{(b-c)!(a-b+c)!}\dfrac{(a-b+c)!}{c!(a-c)!} \]
    \[ = \dfrac{a!}{(b-c)!(a-b)!c!} = \comb{a}{b} \times \comb{b}{c} \]
    completing the proof. \\

    \section*{Exercise 26}
    Proof that all odd integers are the difference of two squares: \\
    Suppose that $a \in \zbb$
    such that $a$ is odd.
    Then $a = 2n+1$ for some $n \in \zbb$.
    Consider now the squares $n^2$ and $(n+1)^2$.
    We know that $(n+1)^2 - n^2 = n^2 + 2n + 1 - n^2 = 2n+1$.
    So any arbitrary odd integer can be written
    as the difference of two squares. \\

    \section*{Exercise 27}
    Proof that for $a, b \in \nbb$,
    if $\gcd(a, b) \geqslant 1$,
    then $b \mid a$ or $b$ is composite: \\
    Suppose that $a, b \in \nbb$
    such that $\gcd(a, b) > 1$.
    We know that $b$ is either prime or composite,
    so if we check the proposition for each case
    we will have covered all of our bases. \\
    If $b$ is prime,
    then no number aside from $b$ and $1$ can divide $b$.
    Since $\gcd(a, b) \mid b$,
    and $\gcd(a, b) > 1$,
    it must be that $\gcd(a, b) = b$.
    Since $\gcd(a, b) \mid a$,
    we conclude that $b \mid a$. \\
    Otherwise, if $b$ is composite,
    then the proposition is true and we can stop here. \\

    \section*{Exercise 28 $***$}
    Proof that if $a, b, c \in \zbb$,
    then $\gcd(a, b) \leqslant \gcd(ca, cb)$: \\
    Suppose that $a, b, c \in \zbb$.
    Take $d = \gcd(a, b)$.
    Then $d \mid a$ and $d \mid b$,
    which means that $a = nd$ and $b = md$
    for some $n, m \in \zbb$.
    This means that $ca = (cn)d$ and $cb = (cm)d$,
    which means that $d \mid ca$ and $d \mid cb$.
    By definition,
    $\gcd(ca, cb)$
    is the largest number that divides both $ca$ and $cb$,
    so since $d$ divides both,
    it is at most equal to it.
    So $\gcd(a, c) \leqslant \gcd(ca, cb)$. \\




\end{document}
